Changing tests

SingleSorted/KAT.thy
@@ -1,179 +1,71 @@
 theory KAT
-  imports Algebras 
+  imports Kleene_Algebra_Left Tests
 begin
 
-class KAT = kleene_algebra +
-  fixes   test_operator :: "'a \<Rightarrow> 'a" ("t_" [100] 101)
-  and     comp_operator :: "'a \<Rightarrow> 'a" ("n_" [90] 91)
-
-  assumes test_mult_idem:   "t x \<cdot> t x = t x"
-  and     test_mult:        "t (t x \<cdot> t y) = t y \<cdot> t x" 
-  and     test_one:         "t 1 = 1"
-  and     test_zero:        "t 0 = 0"
-
-  and     test_mult_comp:   "n x \<cdot> n n x = 0"
-  and     test_de_morgan:   "n x + n y = n (n n x \<cdot> n n y)"
-
-  and     test_comp_closed: "t (n x) = n (t x)"
-  and     test_double_comp: "t x = n n x"
+class kat_zerol = kleene_algebra_zerol + dioid_tests
 begin
 
-lemma test_proj: "t t x = t x"
-  by (metis test_mult test_mult_idem)
-
-lemma test_mult_comm: "t x \<cdot> t y = t y \<cdot> t x"
-  by (metis test_mult test_proj)
-
-lemma test_add_closed: "t (t x + t y) = t x + t y"
-  by (metis add_comm test_de_morgan test_double_comp test_mult)
-
-lemma test_add_comp: "n x + n n x = 1"
-  by (metis mult_oner test_double_comp test_de_morgan test_mult_comp test_one)
-
-lemma test_add_assoc: "t x + (t y + t z) = (t x + t y) + t z" 
-  by (metis add_assoc)
-
-lemma test_add_comm: "t x + t y = t y + t x"
-  by (metis add_comm)
-
-lemma test_add_zerol: "0 + t x = t x"
-  by (metis add_zerol)
-
-lemma test_add_zeror: "t x + 0 = t x"
-  by (metis add_zeror)
-
-lemma test_add_distl: "(t x \<cdot> t y) + t z = (t x + t z) \<cdot> (t y + t z)"
-proof -
-  have one: "(t x \<cdot> t y) + t z \<le> (t x + t z) \<cdot> (t y + t z)"
-    by (metis add_lub mult_double_iso order_refl test_mult_idem)
-  have "t x \<cdot> t y + t x \<cdot> t z \<le>  (t x \<cdot> t y) + t z"
-    by (metis (mono_tags) add_comm add_iso add_ub mult_isor mult_oner test_add_comp test_double_comp test_mult_comm)
-  moreover have "t z \<cdot> t y + t z \<le> (t x \<cdot> t y) + t z"
-    by (metis add_comm add_ub leq_def mult_oner subdistr test_add_comp test_double_comp)
-  moreover have  "(t x + t z) \<cdot> (t y + t z) = (t x \<cdot> t y + t x \<cdot> t z) + (t z \<cdot> t y + t z)"
-    by (metis mult_distr mult_distl test_mult_idem)
-  ultimately have two: "(t x + t z) \<cdot> (t y + t z) \<le> (t x \<cdot> t y) + t z"
-    by (metis add_lub)
-  show ?thesis
-    by (metis eq_iff one two)
+lemma star_sim_right: "\<lbrakk>test b; b\<cdot>q = q\<cdot>b\<rbrakk> \<Longrightarrow> b\<cdot>q\<^sup>\<star> = (b\<cdot>q)\<^sup>\<star>\<cdot>b"
+proof - 
+  assume tb: "test b" and comm: "b\<cdot>q = q\<cdot>b"
+  hence comm2: "b\<cdot>q = b\<cdot>q\<cdot>b"
+    by (metis mult_assoc test_mult_idem_var)
+  moreover hence "b + (b\<cdot>q)\<^sup>\<star>\<cdot>b\<cdot>q = (1 + (b\<cdot>q)\<^sup>\<star>\<cdot>b\<cdot>q)\<cdot>b"
+    by (metis distrib_right' mult_assoc mult_onel)
+  moreover hence "... = (b\<cdot>q)\<^sup>\<star>\<cdot>b"
+    by (metis star_prod_unfold star_slide)
+  ultimately have "b\<cdot>q\<^sup>\<star> \<le> (b\<cdot>q)\<^sup>\<star>\<cdot>b"
+    by (metis order_refl star_sim2)
+  thus ?thesis
+    by (metis comm2 eq_iff star_sim1)
 qed
 
-lemma test_add_distr: "t x + (t y \<cdot> t z) = (t x + t y) \<cdot> (t x + t z)"
-  by (metis add_comm test_add_distl)
+lemma star_sim_left: "\<lbrakk>test b; b\<cdot>q = q\<cdot>b\<rbrakk> \<Longrightarrow> b\<cdot>q\<^sup>\<star> = b\<cdot>(q\<cdot>b)\<^sup>\<star>"
+  by (metis star_sim_right star_slide)
 
-lemma test_mult_assoc: "t x \<cdot> (t y \<cdot> t z) = (t x \<cdot> t y) \<cdot> t z"
-  by (metis mult_assoc)
+lemma comm_star: "\<lbrakk>test b; b\<cdot>p = p\<cdot>b; b\<cdot>q = q\<cdot>b\<rbrakk> \<Longrightarrow> b\<cdot>p\<cdot>(b\<cdot>q)\<^sup>\<star> = b\<cdot>p\<cdot>q\<^sup>\<star>"
+  by (metis star_sim_right mult_assoc star_slide)
 
-lemma test_mult_onel: "1 \<cdot> t x = t x"
-  by (metis mult_onel)
+end
 
-lemma test_mult_oner: "t x \<cdot> 1 = t x"
-  by (metis mult_oner)
+text {*
+  Kleene Algebra with Tests is defined with an embedded Boolean Algebra.
+*}
 
-lemma test_mult_distl: "t x \<cdot> (t y + t z) = (t x \<cdot> t y) + (t x \<cdot> t z)"
-  by (metis mult_distl)
+class kat = kleene_algebra + dioid_tests
+begin
 
-lemma test_mult_distr: "(t x + t y) \<cdot> t z = (t x \<cdot> t z) + (t y \<cdot> t z)"
-  by (metis mult_distr)
-  
-definition test :: "'a \<Rightarrow> bool" where
-  "test x \<equiv> t x = x"
+subclass kat_zerol
+  apply (unfold_locales)
+  by (metis star_inductr)
 
-lemma test_mult_closed: "\<lbrakk>test x; test y\<rbrakk> \<Longrightarrow> test (x \<cdot> y)"
-  by (metis test_def test_mult test_mult_comm)
-
-lemma test_under_one: "test x \<Longrightarrow> x \<le> 1"
-  by (metis order_prop test_add_comp test_def test_double_comp)
-
-lemma test_zero_var: "test 0"
-  by (metis test_def test_zero)
-
-lemma test_one_var: "test 1"
-  by (metis test_def test_one)
-
-lemma test_not_one: "n 1 = 0"
-  by (metis mult_oner test_double_comp test_mult_comp test_one)
-
-lemma test_mult_idem_var: "test x \<Longrightarrow> x \<cdot> x = x"
-  by (metis test_def test_mult_idem)
-
-lemma test_mult_comm_var: "\<lbrakk>test x; test y\<rbrakk> \<Longrightarrow> x \<cdot> y = y \<cdot> x"
-  by (metis test_def test_mult_comm)
-
-lemma test_absorb1: "\<lbrakk>test x; test y\<rbrakk> \<Longrightarrow> x + x \<cdot> y = x"
-  by (metis add_comm leq_def mult_isor mult_oner test_under_one)
-
-lemma test_absorb2: "\<lbrakk>test x; test y\<rbrakk> \<Longrightarrow> x \<cdot> (x + y) = x"
-  by (metis mult_distl test_absorb1 test_def test_mult_idem)
-
-lemma test_leq_mult_def: "\<lbrakk>test x; test y\<rbrakk> \<Longrightarrow> (x \<le> y) = (x \<cdot> y = x)"
-  by (metis add_comm join_plus_equiv leq_def_join test_absorb1 test_absorb2 test_mult_comm_var)
-
-lemma test_double_comp_var: "test x \<Longrightarrow> x = n n x"
-  by (metis test_def test_double_comp)
-
-lemma test_comp: "test x \<Longrightarrow> \<exists>y. x + y = 1 \<and> x \<cdot> y = 0"
-  by (metis test_add_comp test_def test_double_comp test_mult_comp)
-
-lemma test_comp_uniq: "test x \<Longrightarrow> \<exists>!y. x + y = 1 \<and> x \<cdot> y = 0"
-   apply (safe, metis test_comp)
-   by (metis add_zerol mult_distl mult_distr mult_onel test_add_comp test_def test_double_comp test_mult_comp)
-
-lemma test_comp_closed_var: "test x \<Longrightarrow> test (n x)"
-  by (metis test_comp_closed test_def)
-
-lemma test_add_closed_var: "test x \<and> test y \<Longrightarrow> test (x + y)"
-  by (metis test_add_closed test_def)
-
-lemma de_morgan1: "\<lbrakk>test x; test y\<rbrakk> \<Longrightarrow> n x + n y = n (x \<cdot> y)"
-  by (metis test_de_morgan test_def test_double_comp)
-
-lemma de_morgan2: "\<lbrakk>test x; test y\<rbrakk> \<Longrightarrow> n x \<cdot> n y = n (x + y)"
-  by (smt de_morgan1 test_comp_closed_var test_comp_uniq test_double_comp test_double_comp_var test_mult_closed test_mult_comm_var test_not_one)
-
-lemma test_comp_anti: "\<lbrakk>test x; test y\<rbrakk> \<Longrightarrow> (x \<le> y) = (n y \<le> n x)"
-  by (metis add_comm de_morgan1 de_morgan2 join_plus_equiv test_absorb1 test_def test_double_comp test_leq_mult_def)
-
-lemma ba_1: "\<lbrakk>test x; test y; test z\<rbrakk> \<Longrightarrow> x + y + n y = z + n z"
-  by (metis add_assoc mult_onel test_absorb1 test_add_comp test_def test_double_comp test_one_var)
-
-lemma ba2: "\<lbrakk>test x; test y\<rbrakk> \<Longrightarrow> x + x = x + n (y + n y)"
-  by (metis add_idem add_zeror ba_1 test_not_one test_one_var)
-
-lemma ba3: "\<lbrakk>test x; test y\<rbrakk> \<Longrightarrow> x = (x \<cdot> y) + (x \<cdot> n y)"
-  by (metis mult_distl mult_oner test_add_comp test_def test_double_comp)
-
-lemma ba4: "\<lbrakk>test x; test y\<rbrakk> \<Longrightarrow> x = (x + n y) \<cdot> (x + y)"
-proof -
-  assume assm: "test x" "test y"
-  hence "(x + n y) \<cdot> (x + y) = (x + x \<cdot> y) + (n y \<cdot> x + n y \<cdot> y)"
-    by (metis mult_distr mult_distl test_mult_idem_var)
-  moreover have "... = x + x \<cdot> y + n y \<cdot> x"
-    by (metis add_zeror assm(2) test_double_comp_var test_mult_comp)
-  moreover have "... = x"
-    by (metis add_assoc add_idem assm mult_distl mult_oner test_add_comp test_def test_double_comp test_mult_comm_var)
-  ultimately show ?thesis
-    by metis
-qed
-
-lemma ba5: "\<lbrakk>test x; test y\<rbrakk> \<Longrightarrow> (x + y) \<cdot> n x = y \<cdot> n x"
-  by (metis (hide_lams, no_types) add_comm add_zeror ba4 mult_distr test_comp_closed_var test_comp_uniq test_mult_comm_var test_zero_var)
-
-lemma ba6: "test x \<Longrightarrow> n x \<cdot> x = 0"
-  by (metis test_def test_double_comp test_mult_comp)
-
-lemma ba7: "\<lbrakk>test x; test y\<rbrakk> \<Longrightarrow> n x = n (x + y) + n (x + n y)"
-  by (metis ba3 de_morgan2 test_comp_closed_var test_double_comp test_double_comp_var)
-
-lemma kat_eq1: "\<lbrakk>test p; test q\<rbrakk> \<Longrightarrow> (p \<cdot> x \<cdot> n q = 0) = (p \<cdot> x \<le> x \<cdot> q)"
+lemma kat_eq1: "\<lbrakk>test p; test q\<rbrakk> \<Longrightarrow> (p\<cdot>x\<cdot>!q = 0) = (p\<cdot>x = p\<cdot>x\<cdot>q)"
   apply default
-  apply (metis add_comm add_zerol ba3 mult_distl mult_isol mult_onel mult_oner test_one_var test_under_one)
-  by (metis (hide_lams, no_types) ba6 eq_iff min_zero mult_annir mult_assoc mult_isol test_comp_closed_var test_double_comp_var)
+  apply (subgoal_tac "p \<cdot> x = p \<cdot> x \<cdot> (q + ! q)")
+  apply (metis add_0_left add_commute distrib_left)
+  apply (metis mult_1_right test_add_comp test_def)
+  by (metis annir test_double_comp_var test_mult_comp mult_assoc)
 
-lemma kat_eq2: "\<lbrakk>test p; test q\<rbrakk> \<Longrightarrow> (p \<cdot> x \<cdot> n q = 0) = (p \<cdot> x = p \<cdot> x \<cdot> q)"
+lemma kat_eq2: "\<lbrakk>test p; test q\<rbrakk> \<Longrightarrow> (p\<cdot>x\<cdot>!q = 0) = (p\<cdot>x \<le> x\<cdot>q)"
   apply default
-  apply (metis add_zerol ba3 mult_distl mult_onel mult_oner test_comp_closed_var test_double_comp_var test_one_var)
-  by (metis mult_annir mult_assoc test_def test_double_comp test_mult_comp)
+  apply (metis add_idem' kat_eq1 less_eq_def mult_1_left mult_assoc star_inductl_var_equiv star_subid test_ub_var)
+  apply (subgoal_tac "p \<cdot> x \<cdot> ! q \<le> x \<cdot> q \<cdot> ! q")
+  apply (metis annir test_double_comp_var test_mult_comp mult_assoc zero_unique)
+  by (metis mult_isor)
+
+text {* 
+  Some commutativity conditions equivalence lemmas 
+*}
+lemma comm_eq1: "test b \<Longrightarrow> (p\<cdot>b = b\<cdot>p) = (b\<cdot>p\<cdot>!b + !b\<cdot>p\<cdot>b = 0)"
+  apply default
+  apply (metis add_0_left annil annir test_double_comp_var test_mult_comp mult_assoc)
+  by (metis add_0_left ba6 de_morgan1 distrib_right' test_double_comp_var kat_eq1 test_one mult_assoc mult_onel no_trivial_inverse test_comp_closed_var test_not_one)
+
+lemma comm_eq2: "test b \<Longrightarrow> (p\<cdot>!b = !b\<cdot>p) = (b\<cdot>p\<cdot>!b + !b\<cdot>p\<cdot>b = 0)"
+  by (metis add_comm comm_eq1 test_comp_closed_var test_double_comp_var)
+
+lemma comm_eq3: "test b \<Longrightarrow> (p\<cdot>b = b\<cdot>p) = (p\<cdot>!b = !b\<cdot>p)"
+  by (metis comm_eq1 comm_eq2)
 
 end
 
