SingleSorted/FolkTheorem.thy
@@ -2,119 +2,14 @@ theory FolkTheorem
   imports KAT
 begin
 
-context KAT begin
-
-notation comp_operator ("!_" [101] 100)
-
-text {* 
-  Kleene algebra star sliding and denesting 
-*}
-theorem star_sliding: "p\<cdot>(q\<cdot>p)\<^sup>* = (p\<cdot>q)\<^sup>*\<cdot>p"
-  by (metis star_slide)
-
-lemma star_denesting1: "(p + q)\<^sup>* \<le> p\<^sup>*\<cdot>(q\<cdot>p\<^sup>*)\<^sup>*"
-proof -
-  have "1 \<le> p\<^sup>*\<cdot>(q\<cdot>p\<^sup>*)\<^sup>*"
-    by (metis add_lub mult_onel star_def subdistl)
-  moreover have "p\<cdot>p\<^sup>*\<cdot>(q\<cdot>p\<^sup>*)\<^sup>* \<le> p\<^sup>*\<cdot>(q\<cdot>p\<^sup>*)\<^sup>*"
-    by (metis mult_isol star_1l)
-  moreover have "q\<cdot>p\<^sup>*\<cdot>(q\<cdot>p\<^sup>*)\<^sup>* \<le> p\<^sup>*\<cdot>(q\<cdot>p\<^sup>*)\<^sup>*"
-    by (metis mult_isol mult_onel one_le_star order_trans star_1l)
-  moreover have "1 + (p + q)\<cdot>p\<^sup>*\<cdot>(q\<cdot>p\<^sup>*)\<^sup>* \<le> 1 + p\<cdot>p\<^sup>*\<cdot>(q\<cdot>p\<^sup>*)\<^sup>* + q\<cdot>p\<^sup>*\<cdot>(q\<cdot>p\<^sup>*)\<^sup>*"
-    by (metis add_assoc mult_distr order_refl)
-  ultimately have "... \<le> p\<^sup>*\<cdot>(q\<cdot>p\<^sup>*)\<^sup>*"
-    by (metis add_lub)
-  thus ?thesis
-    by (metis add_assoc mult_assoc mult_distr mult_oner star_inductl)
-qed
-
-lemma star_denesting2: "p\<^sup>*\<cdot>(q\<cdot>p\<^sup>*)\<^sup>* \<le> (p + q)\<^sup>*"
-proof -
-  have "p\<^sup>*\<cdot>(q\<cdot>p\<^sup>*)\<^sup>* \<le> (p + q)\<^sup>*\<cdot>((p + q)\<cdot>(p + q)\<^sup>*)\<^sup>*"
-    by (metis add_comm add_ub mult_double_iso star_iso)
-  thus ?thesis
-    by (metis star2 star_def star_invol star_trans_eq star_transl)
-qed
-
-theorem star_denesting: "p\<^sup>*\<cdot>(q\<cdot>p\<^sup>*)\<^sup>* = (p + q)\<^sup>*"
-  by (metis add_comm leq_def star_denesting1 star_denesting2)
-
-lemma ka_denesting: "(p\<^sup>* \<cdot> q)\<^sup>* = 1 + (p+q)\<^sup>*\<cdot>q"
-  by (metis mult_assoc star_def star_denesting star_slide star_transl)
-
-lemma kat_double: "\<lbrakk>test b; test c\<rbrakk> \<Longrightarrow> b\<cdot>c\<cdot>b\<cdot>p = b\<cdot>c\<cdot>p"
-  by (metis (full_types) mult_assoc test_mult_comm_var test_mult_idem_var)
-
-lemma kat_double_zero1: "\<lbrakk>test b; test c\<rbrakk> \<Longrightarrow> b\<cdot>c\<cdot>!b\<cdot>p = 0"
-  by (metis mult_annil mult_assoc test_double_comp_var test_mult_comm_var test_mult_comp)
-
-lemma kat_double_zero2: "\<lbrakk>test b; test c\<rbrakk> \<Longrightarrow> !b\<cdot>c\<cdot>b\<cdot>p = 0"
-  by (metis kat_double_zero1 test_comp_closed_var test_double_comp_var)
-
-
-text {* 
-  Some commutativity conditions equivalence lemmas 
-*}
-lemma comm_eq1: "test b \<Longrightarrow> (p\<cdot>b = b\<cdot>p) = (b\<cdot>p\<cdot>!b + !b\<cdot>p\<cdot>b = 0)"
-proof (default, metis add_zerol ba6 eq_refl kat_eq1 mult_annil mult_assoc)
-  assume tb: "test b" and assm: "b\<cdot>p\<cdot>!b + !b\<cdot>p\<cdot>b = 0"
-  have "p\<cdot>b = (b + !b)\<cdot>p\<cdot>b"
-    by (metis mult_onel tb test_add_comp test_double_comp_var)
-  moreover hence "... = b\<cdot>p\<cdot>b"
-    by (metis add_comm add_ub add_zeror assm eq_iff mult_assoc mult_distr)
-  moreover have "b\<cdot>p = b\<cdot>p\<cdot>(b + !b)"
-    by (metis mult_oner tb test_add_comp test_double_comp_var)
-  moreover hence "... = b\<cdot>p\<cdot>b"
-    by (metis add_comm add_ub add_zerol assm eq_iff mult_assoc mult_distl)
-  ultimately show "p \<cdot> b = b \<cdot> p"
-    by (metis)
-qed
-
-lemma comm_eq2: "test b \<Longrightarrow> (p\<cdot>!b = !b\<cdot>p) = (b\<cdot>p\<cdot>!b + !b\<cdot>p\<cdot>b = 0)"
-  by (metis add_comm comm_eq1 test_comp_closed_var test_double_comp_var)
-
-lemma comm_eq3: "test b \<Longrightarrow> (p\<cdot>b = b\<cdot>p) = (p\<cdot>!b = !b\<cdot>p)"
-  by (metis comm_eq1 comm_eq2)
-
-lemma comm_eq4: "\<lbrakk>test b; b\<cdot>q = q\<cdot>b\<rbrakk> \<Longrightarrow> b\<cdot>q\<^sup>* = (b\<cdot>q)\<^sup>*\<cdot>b"
-proof - 
-  assume tb: "test b" and comm: "b\<cdot>q = q\<cdot>b"
-  hence comm2: "b\<cdot>q = b\<cdot>q\<cdot>b"
-    by (metis mult_assoc test_mult_idem_var)
-  moreover hence "b + (b\<cdot>q)\<^sup>*\<cdot>b\<cdot>q = (1 + (b\<cdot>q)\<^sup>*\<cdot>b\<cdot>q)\<cdot>b"
-    by (metis comm mult_assoc mult_distl mult_oner star_def star_sliding star_transr)
-  moreover hence "... = (b\<cdot>q)\<^sup>*\<cdot>b"
-    by (metis mult_assoc star_def star_transr)
-  ultimately have "b\<cdot>q\<^sup>* \<le> (b\<cdot>q)\<^sup>*\<cdot>b"
-    by (metis order_refl star_sim2)
-  thus ?thesis
-    by (metis comm2 eq_iff star_sim1)
-qed
-
-lemma comm_eq5: "\<lbrakk>test b; b\<cdot>q = q\<cdot>b\<rbrakk> \<Longrightarrow> b\<cdot>q\<^sup>* = q\<^sup>*\<cdot>b"
-  by (metis eq_iff star_sim1 star_sim2)
-
-lemma comm_eq6: "\<lbrakk>test b; b\<cdot>q = q\<cdot>b\<rbrakk> \<Longrightarrow> b\<cdot>q\<^sup>* = b\<cdot>(q\<cdot>b)\<^sup>*"
-  by (metis comm_eq4 star_slide)
-
-lemma comm_add: "\<lbrakk>test b; b\<cdot>p = p\<cdot>b; b\<cdot>q = q\<cdot>b\<rbrakk> \<Longrightarrow> b\<cdot>(p + q) = (p + q)\<cdot>b"
-  by (metis mult_distl mult_distr)
-
-lemma comm_add_var: "\<lbrakk>test b; test c; test e; b\<cdot>p = p\<cdot>b; b\<cdot>q = q\<cdot>b\<rbrakk> \<Longrightarrow> b\<cdot>(c\<cdot>p + e\<cdot>q) = (c\<cdot>p + e\<cdot>q)\<cdot>b"
-  by (metis comm_add mult_assoc test_mult_comm_var)
-
-lemma comm_mult: "\<lbrakk>test b; test c; c\<cdot>p = p\<cdot>c\<rbrakk> \<Longrightarrow> b\<cdot>p\<cdot>c = c\<cdot>b\<cdot>p"
-  by (metis mult_assoc test_mult_comm_var)
-
-lemma comm_star: "\<lbrakk>test b; b\<cdot>p = p\<cdot>b; b\<cdot>q = q\<cdot>b\<rbrakk> \<Longrightarrow> b\<cdot>p\<cdot>(b\<cdot>q)\<^sup>* = b\<cdot>p\<cdot>q\<^sup>*"
-  by (metis comm_eq4 mult_assoc star_slide)
+context kat begin
 
 text {*
-  Some distributivity lemmas
+  Some distributivity helper lemmas
 *}
 
 lemma folk_distr: "(b + c)\<cdot>(p + q) = b\<cdot>p + c\<cdot>p + b\<cdot>q + c\<cdot>q"
-    by (metis add_assoc mult_distl mult_distr)
+    by (metis add_assoc distrib_left distrib_right)
 
 lemma folk_distr2: 
   assumes tb: "test b" and tc: "test c"
@@ -123,35 +18,7 @@ proof -
   have "(b\<cdot>c + !b\<cdot>!c)\<cdot>(b\<cdot>p + !b\<cdot>q) = b\<cdot>c\<cdot>b\<cdot>p + !b\<cdot>!c\<cdot>b\<cdot>p + b\<cdot>c\<cdot>!b\<cdot>q + !b\<cdot>!c\<cdot>!b\<cdot>q"
     by (metis folk_distr mult_assoc)
   thus ?thesis
-    by (metis tb tc kat_double kat_double_zero1 kat_double_zero2 test_comp_closed_var add_zeror)
-qed
-
-lemma folk_de_morgan: "\<lbrakk>test a; test b; test c\<rbrakk> \<Longrightarrow> a\<cdot>b + !a\<cdot>c = (!a + b)\<cdot>(a + c)"
-proof -
-  assume assm: "test a" "test b" "test c"
-  have "(!a + b)\<cdot>(a + c) = b\<cdot>a + !a\<cdot>c + b\<cdot>c"
-    by (metis add_assoc mult_distl mult_distr add_zerol assm(1) test_double_comp_var test_mult_comp)
-  moreover hence "... = b\<cdot>a + !a\<cdot>c + (a + !a)\<cdot>b\<cdot>c"
-    by (metis assm(1) mult_onel test_add_comp test_double_comp_var)
-  ultimately have one: "(!a + b)\<cdot>(a + c) = a\<cdot>b + !a\<cdot>c + a\<cdot>b\<cdot>c + !a\<cdot>b\<cdot>c"
-    by (metis add_assoc mult_distr assm(1,2) test_mult_comm_var)
-  have "a\<cdot>b + !a\<cdot>c = a\<cdot>b\<cdot>(1 + c) + !a\<cdot>c\<cdot>(1 + b)"
-    by (metis assm(2,3) mult_assoc mult_distl mult_oner test_absorb1)
-  hence two: "a\<cdot>b + !a\<cdot>c = a\<cdot>b + !a\<cdot>c + a\<cdot>b\<cdot>c + !a\<cdot>c\<cdot>b"
-    by (metis add_assoc add_comm mult_distl mult_oner)
-  from one and two show ?thesis
-    by (metis assm(2,3) mult_assoc test_mult_comm_var)
-qed
-
-lemma folk_de_morgan2: "\<lbrakk>test a; test b; test c\<rbrakk> \<Longrightarrow> !(a\<cdot>b + !a\<cdot>c) = (a\<cdot>!b + !a\<cdot>!c)"
-proof -
-  assume assm: "test a" "test b" "test c"
-  hence "!(a\<cdot>b + !a\<cdot>c) = !(a\<cdot>b)\<cdot>!(!a\<cdot>c)"
-    by (metis de_morgan2 test_comp_closed_var test_mult_closed)
-  also have "... = (!a + !b)\<cdot>(a + !c)"
-    by (metis assm de_morgan1 test_def test_double_comp)
-  finally show ?thesis
-    by (metis assm folk_de_morgan test_comp_closed_var)
+    by (metis tb tc test2 test3 test4 annil test_comp_closed_var add_zeror)
 qed
 
 text {*
@@ -172,109 +39,110 @@ text {*
 
 lemma conditional_helper1:
   assumes "test b" "test c" "test d" "test e" "test f" "c\<cdot>p = p\<cdot>c" "c\<cdot>q = q\<cdot>c" "c\<cdot>r = r\<cdot>c"
-  shows "b\<cdot>c\<cdot>p\<cdot>(c\<cdot>d\<cdot>q + !c\<cdot>e\<cdot>r)\<^sup>*\<cdot>c\<cdot>f = b\<cdot>c\<cdot>p\<cdot>(d\<cdot>q)\<^sup>*\<cdot>f"
+  shows "b\<cdot>c\<cdot>p\<cdot>(c\<cdot>d\<cdot>q + !c\<cdot>e\<cdot>r)\<^sup>\<star>\<cdot>c\<cdot>f = b\<cdot>c\<cdot>p\<cdot>(d\<cdot>q)\<^sup>\<star>\<cdot>f"
 proof -
   have "c\<cdot>(c\<cdot>d\<cdot>q + !c\<cdot>e\<cdot>r) = (c\<cdot>d\<cdot>q + !c\<cdot>e\<cdot>r)\<cdot>c"
     by (metis assms(2-4,7,8) comm_add_var test_comp_closed_var test_mult_closed)
-  hence "b\<cdot>c\<cdot>p\<cdot>(c\<cdot>d\<cdot>q + !c\<cdot>e\<cdot>r)\<^sup>*\<cdot>c\<cdot>f = b\<cdot>c\<cdot>p\<cdot>c\<cdot>((c\<cdot>d\<cdot>q + !c\<cdot>e\<cdot>r)\<cdot>c)\<^sup>*\<cdot>f"
-    by (smt mult_assoc assms(1-4) test_comp_closed_var mult_assoc comm_eq4 comm_eq5)
-  also have "... = b\<cdot>c\<cdot>p\<cdot>c\<cdot>(c\<cdot>d\<cdot>q\<cdot>c + !c\<cdot>e\<cdot>r\<cdot>c)\<^sup>*\<cdot>f"
-    by (metis mult_distr)
-  also have "... = b\<cdot>c\<cdot>p\<cdot>(c\<cdot>c\<cdot>d\<cdot>q + !c\<cdot>e\<cdot>r\<cdot>c)\<^sup>*\<cdot>f"
-    by (metis assms(2-3,6-8) comm_mult mult_assoc test_mult_idem_var)
-  also have "... = b\<cdot>c\<cdot>p\<cdot>(c\<cdot>c\<cdot>d\<cdot>q + !c\<cdot>c\<cdot>e\<cdot>r)\<^sup>*\<cdot>f"
+  hence "b\<cdot>c\<cdot>p\<cdot>(c\<cdot>d\<cdot>q + !c\<cdot>e\<cdot>r)\<^sup>\<star>\<cdot>c\<cdot>f = b\<cdot>c\<cdot>p\<cdot>c\<cdot>((c\<cdot>d\<cdot>q + !c\<cdot>e\<cdot>r)\<cdot>c)\<^sup>\<star>\<cdot>f"
+    by (smt mult_assoc assms(1-4) test_comp_closed_var mult_assoc star_sim_left star_sim3)
+  also have "... = b\<cdot>c\<cdot>p\<cdot>c\<cdot>(c\<cdot>d\<cdot>q\<cdot>c + !c\<cdot>e\<cdot>r\<cdot>c)\<^sup>\<star>\<cdot>f"
+    by (metis distrib_right)
+  also have "... = b\<cdot>c\<cdot>p\<cdot>(c\<cdot>c\<cdot>d\<cdot>q + !c\<cdot>e\<cdot>r\<cdot>c)\<^sup>\<star>\<cdot>f"
+    by (smt assms(1-3,6,7) comm_mult test_mult_closed test_mult_comm_var test_mult_idem_var)
+  also have "... = b\<cdot>c\<cdot>p\<cdot>(c\<cdot>c\<cdot>d\<cdot>q + !c\<cdot>c\<cdot>e\<cdot>r)\<^sup>\<star>\<cdot>f"
     by (metis assms(2,4,8) comm_mult mult_assoc)
-  also have "... = b\<cdot>c\<cdot>p\<cdot>(c\<cdot>d\<cdot>q)\<^sup>*\<cdot>f"
-    by (metis ba6 assms(2) mult_annil test_mult_idem_var add_zeror)
+  also have "... = b\<cdot>c\<cdot>p\<cdot>(c\<cdot>d\<cdot>q)\<^sup>\<star>\<cdot>f"
+    by (metis add_0_left add_commute assms(2) comm_eq1 mult_1_left mult_1_right no_trivial_inverse test_one_var test_mult_idem_var)
   finally show ?thesis
     by (smt assms comm_star comm_mult mult_assoc)
 qed
 
 lemma conditional_helper2: 
   assumes "test b" "test c" "test d" "test e" "test f" "c\<cdot>p = p\<cdot>c" "c\<cdot>q = q\<cdot>c" "c\<cdot>r = r\<cdot>c"
-  shows "b\<cdot>c\<cdot>p\<cdot>(c\<cdot>d\<cdot>q + !c\<cdot>e\<cdot>r)\<^sup>*\<cdot>!c\<cdot>f = 0"
+  shows "b\<cdot>c\<cdot>p\<cdot>(c\<cdot>d\<cdot>q + !c\<cdot>e\<cdot>r)\<^sup>\<star>\<cdot>!c\<cdot>f = 0"
 proof -
   have "!c\<cdot>(c\<cdot>d\<cdot>q + !c\<cdot>e\<cdot>r) = (c\<cdot>d\<cdot>q + !c\<cdot>e\<cdot>r)\<cdot>!c"
     by (metis assms(2-4,7,8) comm_add_var comm_eq3 test_comp_closed_var test_mult_closed)
-  hence "b\<cdot>c\<cdot>p\<cdot>(c\<cdot>d\<cdot>q + !c\<cdot>e\<cdot>r)\<^sup>*\<cdot>!c\<cdot>f = b\<cdot>c\<cdot>p\<cdot>!c\<cdot>((c\<cdot>d\<cdot>q + !c\<cdot>e\<cdot>r)\<cdot>!c)\<^sup>*\<cdot>f"
-    by (smt mult_assoc assms(1-4) test_comp_closed_var mult_assoc comm_eq4 comm_eq5)
-  also have "... = b\<cdot>c\<cdot>!c\<cdot>p\<cdot>((c\<cdot>d\<cdot>q + !c\<cdot>e\<cdot>r)\<cdot>!c)\<^sup>*\<cdot>f"
+  hence "b\<cdot>c\<cdot>p\<cdot>(c\<cdot>d\<cdot>q + !c\<cdot>e\<cdot>r)\<^sup>\<star>\<cdot>!c\<cdot>f = b\<cdot>c\<cdot>p\<cdot>!c\<cdot>((c\<cdot>d\<cdot>q + !c\<cdot>e\<cdot>r)\<cdot>!c)\<^sup>\<star>\<cdot>f"
+    by (smt mult_assoc assms(1-4) test_comp_closed_var mult_assoc star_sim_right star_sim3)
+  also have "... = b\<cdot>c\<cdot>!c\<cdot>p\<cdot>((c\<cdot>d\<cdot>q + !c\<cdot>e\<cdot>r)\<cdot>!c)\<^sup>\<star>\<cdot>f"
     by (metis assms(2,6) comm_eq3 mult_assoc)
   finally show ?thesis using assms
-    by (metis mult_annil mult_assoc test_double_comp_var test_mult_comp)
+    by (metis add_0_left add_commute assms(2) comm_eq1 mult_1_left mult_1_right no_trivial_inverse test_one_var annil mult_assoc)
 qed
 
 lemma conditional_helper3:
   assumes "test b" "test c" "test d" "test e" "test f" "c\<cdot>p = p\<cdot>c" "c\<cdot>q = q\<cdot>c" "c\<cdot>r = r\<cdot>c"
-  shows "!b\<cdot>!c\<cdot>p\<cdot>(c\<cdot>d\<cdot>q + !c\<cdot>e\<cdot>r)\<^sup>*\<cdot>!c\<cdot>!f = !b\<cdot>!c\<cdot>p\<cdot>(e\<cdot>r)\<^sup>*\<cdot>!f"
+  shows "!b\<cdot>!c\<cdot>p\<cdot>(c\<cdot>d\<cdot>q + !c\<cdot>e\<cdot>r)\<^sup>\<star>\<cdot>!c\<cdot>!f = !b\<cdot>!c\<cdot>p\<cdot>(e\<cdot>r)\<^sup>\<star>\<cdot>!f"
 proof -
   have comm: "!c\<cdot>p = p\<cdot>!c" "!c\<cdot>q = q\<cdot>!c" "!c\<cdot>r = r\<cdot>!c"
     by (metis assms comm_eq3)+
   have "c\<cdot>(c\<cdot>d\<cdot>q + !c\<cdot>e\<cdot>r) = (c\<cdot>d\<cdot>q + !c\<cdot>e\<cdot>r)\<cdot>c"
     by (metis assms(2-4,7,8) comm_add_var test_comp_closed_var test_mult_closed)
-  hence "!b\<cdot>!c\<cdot>p\<cdot>(c\<cdot>d\<cdot>q + !c\<cdot>e\<cdot>r)\<^sup>*\<cdot>!c\<cdot>!f = !b\<cdot>!c\<cdot>p\<cdot>!c\<cdot>((c\<cdot>d\<cdot>q + !c\<cdot>e\<cdot>r)\<cdot>!c)\<^sup>*\<cdot>!f"
-    by (smt mult_assoc assms(1-4) test_comp_closed_var mult_assoc comm_eq3 comm_eq4 comm_eq5)
-  also have "... = !b\<cdot>!c\<cdot>p\<cdot>!c\<cdot>(c\<cdot>d\<cdot>q\<cdot>!c + !c\<cdot>e\<cdot>r\<cdot>!c)\<^sup>*\<cdot>!f"
-    by (metis mult_distr)
-  also have "... = !b\<cdot>!c\<cdot>!c\<cdot>p\<cdot>(c\<cdot>!c\<cdot>d\<cdot>q + !c\<cdot>e\<cdot>r\<cdot>!c)\<^sup>*\<cdot>!f"
+  hence "!b\<cdot>!c\<cdot>p\<cdot>(c\<cdot>d\<cdot>q + !c\<cdot>e\<cdot>r)\<^sup>\<star>\<cdot>!c\<cdot>!f = !b\<cdot>!c\<cdot>p\<cdot>!c\<cdot>((c\<cdot>d\<cdot>q + !c\<cdot>e\<cdot>r)\<cdot>!c)\<^sup>\<star>\<cdot>!f"
+    by (smt mult_assoc assms(1-4) test_comp_closed_var mult_assoc comm_eq3 star_sim_right star_sim3)
+  also have "... = !b\<cdot>!c\<cdot>p\<cdot>!c\<cdot>(c\<cdot>d\<cdot>q\<cdot>!c + !c\<cdot>e\<cdot>r\<cdot>!c)\<^sup>\<star>\<cdot>!f"
+    by (metis distrib_right)
+  also have "... = !b\<cdot>!c\<cdot>!c\<cdot>p\<cdot>(c\<cdot>!c\<cdot>d\<cdot>q + !c\<cdot>e\<cdot>r\<cdot>!c)\<^sup>\<star>\<cdot>!f"
     by (metis assms(2,3) comm(1,2) comm_mult mult_assoc test_comp_closed_var)
-  also have "... = !b\<cdot>!c\<cdot>!c\<cdot>p\<cdot>(c\<cdot>!c\<cdot>d\<cdot>q + !c\<cdot>!c\<cdot>e\<cdot>r)\<^sup>*\<cdot>!f"
+  also have "... = !b\<cdot>!c\<cdot>!c\<cdot>p\<cdot>(c\<cdot>!c\<cdot>d\<cdot>q + !c\<cdot>!c\<cdot>e\<cdot>r)\<^sup>\<star>\<cdot>!f"
     by (metis assms(2,4) comm(1,3) comm_mult mult_assoc test_comp_closed_var)
-  also have "... = !b\<cdot>!c\<cdot>p\<cdot>((c\<cdot>!c)\<cdot>d\<cdot>q + !c\<cdot>e\<cdot>r)\<^sup>*\<cdot>!f"
-    by (metis assms(2) mult_assoc test_comp_closed_var test_mult_idem_var)
-  also have "... = !b\<cdot>!c\<cdot>p\<cdot>(!c\<cdot>e\<cdot>r)\<^sup>*\<cdot>!f"
-    by (metis assms(2) mult_annil test_double_comp_var test_mult_comp add_zerol)
+  also have "... = !b\<cdot>!c\<cdot>p\<cdot>((c\<cdot>!c)\<cdot>d\<cdot>q + !c\<cdot>e\<cdot>r)\<^sup>\<star>\<cdot>!f"
+    by (smt assms(2) test_mult_idem_var mult_assoc test_comp_closed_var)
+  also have "... = !b\<cdot>!c\<cdot>p\<cdot>(!c\<cdot>e\<cdot>r)\<^sup>\<star>\<cdot>!f"
+    by (smt add_comm assms(2-5) calculation comm comm_mult conditional_helper1 test_double_comp_var test_mult_idem_var mult_assoc test_comp_closed_var)
   finally show ?thesis
     by (smt assms comm comm_star comm_mult mult_assoc test_comp_closed_var)
 qed
 
 lemma conditional_helper4: 
   assumes "test b" "test c" "test d" "test e" "test f" "c\<cdot>p = p\<cdot>c" "c\<cdot>q = q\<cdot>c" "c\<cdot>r = r\<cdot>c"
-  shows "!b\<cdot>!c\<cdot>p\<cdot>(c\<cdot>d\<cdot>q + !c\<cdot>e\<cdot>r)\<^sup>*\<cdot>c\<cdot>!f = 0"
+  shows "!b\<cdot>!c\<cdot>p\<cdot>(c\<cdot>d\<cdot>q + !c\<cdot>e\<cdot>r)\<^sup>\<star>\<cdot>c\<cdot>!f = 0"
 proof -
   have comm: "!c\<cdot>p = p\<cdot>!c" "!c\<cdot>q = q\<cdot>!c" "!c\<cdot>r = r\<cdot>!c"
     by (metis assms comm_eq3)+
   have "!c\<cdot>(c\<cdot>d\<cdot>q + !c\<cdot>e\<cdot>r) = (c\<cdot>d\<cdot>q + !c\<cdot>e\<cdot>r)\<cdot>!c" using comm_add_var
     by (metis assms(2-4,7,8) comm_eq3 test_comp_closed_var test_mult_closed)
-  hence "!b\<cdot>!c\<cdot>p\<cdot>(c\<cdot>d\<cdot>q + !c\<cdot>e\<cdot>r)\<^sup>*\<cdot>c\<cdot>!f = !b\<cdot>!c\<cdot>p\<cdot>c\<cdot>((c\<cdot>d\<cdot>q + !c\<cdot>e\<cdot>r)\<cdot>c)\<^sup>*\<cdot>!f"
-    by (smt mult_assoc assms test_comp_closed_var mult_assoc comm_eq3 comm_eq4 comm_eq5)
-  also have "... = !b\<cdot>!c\<cdot>c\<cdot>p\<cdot>((c\<cdot>d\<cdot>q + !c\<cdot>e\<cdot>r)\<cdot>c)\<^sup>*\<cdot>!f"
+  hence "!b\<cdot>!c\<cdot>p\<cdot>(c\<cdot>d\<cdot>q + !c\<cdot>e\<cdot>r)\<^sup>\<star>\<cdot>c\<cdot>!f = !b\<cdot>!c\<cdot>p\<cdot>c\<cdot>((c\<cdot>d\<cdot>q + !c\<cdot>e\<cdot>r)\<cdot>c)\<^sup>\<star>\<cdot>!f"
+    by (smt mult_assoc assms test_comp_closed_var mult_assoc comm_eq3 star_sim_right star_sim3)
+  also have "... = !b\<cdot>!c\<cdot>c\<cdot>p\<cdot>((c\<cdot>d\<cdot>q + !c\<cdot>e\<cdot>r)\<cdot>c)\<^sup>\<star>\<cdot>!f"
     by (metis assms(2,6) comm_eq3 mult_assoc)
   finally show ?thesis using assms
-    by (metis mult_annil mult_assoc test_double_comp_var test_mult_comp)
+    by (smt add_comm comm(1) comm(2) comm(3) conditional_helper2 test_double_comp_var test_comp_closed_var)
+
 qed
 
 theorem conditional: 
   assumes "test b" "test c" "test d1" "test d2" "c\<cdot>p1 = p1\<cdot>c" "c\<cdot>p2 = p2\<cdot>c" "c\<cdot>q1 = q1\<cdot>c" "c\<cdot>q2 = q2\<cdot>c"
-  shows "(b\<cdot>c + !b\<cdot>!c)\<cdot>(b\<cdot>p1\<cdot>(d1\<cdot>q1)\<^sup>*\<cdot>!d1 + !b\<cdot>p2\<cdot>(d2\<cdot>q2)\<^sup>*\<cdot>!d2) = 
-      (b\<cdot>c + !b\<cdot>!c)\<cdot>(c\<cdot>p1 + !c\<cdot>p2)\<cdot>((c\<cdot>d1 + !c\<cdot>d2)\<cdot>(c\<cdot>q1 + !c\<cdot>q2))\<^sup>*\<cdot>!(c\<cdot>d1 + !c\<cdot>d2)"
+  shows "(b\<cdot>c + !b\<cdot>!c)\<cdot>(b\<cdot>p1\<cdot>(d1\<cdot>q1)\<^sup>\<star>\<cdot>!d1 + !b\<cdot>p2\<cdot>(d2\<cdot>q2)\<^sup>\<star>\<cdot>!d2) = 
+      (b\<cdot>c + !b\<cdot>!c)\<cdot>(c\<cdot>p1 + !c\<cdot>p2)\<cdot>((c\<cdot>d1 + !c\<cdot>d2)\<cdot>(c\<cdot>q1 + !c\<cdot>q2))\<^sup>\<star>\<cdot>!(c\<cdot>d1 + !c\<cdot>d2)"
 proof -
-  have lhs: "(b\<cdot>c + !b\<cdot>!c)\<cdot>(b\<cdot>p1\<cdot>(d1\<cdot>q1)\<^sup>*\<cdot>!d1 + !b\<cdot>p2\<cdot>(d2\<cdot>q2)\<^sup>*\<cdot>!d2) = b\<cdot>c\<cdot>(p1\<cdot>(d1\<cdot>q1)\<^sup>*\<cdot>!d1) + !b\<cdot>!c\<cdot>(p2\<cdot>(d2\<cdot>q2)\<^sup>*\<cdot>!d2)"
+  have lhs: "(b\<cdot>c + !b\<cdot>!c)\<cdot>(b\<cdot>p1\<cdot>(d1\<cdot>q1)\<^sup>\<star>\<cdot>!d1 + !b\<cdot>p2\<cdot>(d2\<cdot>q2)\<^sup>\<star>\<cdot>!d2) = b\<cdot>c\<cdot>(p1\<cdot>(d1\<cdot>q1)\<^sup>\<star>\<cdot>!d1) + !b\<cdot>!c\<cdot>(p2\<cdot>(d2\<cdot>q2)\<^sup>\<star>\<cdot>!d2)"
     by (metis assms(1,2) mult_assoc folk_distr2)
   have "(b\<cdot>c + !b\<cdot>!c)\<cdot>(c\<cdot>p1 + !c\<cdot>p2) = b\<cdot>c\<cdot>p1 + !b\<cdot>!c\<cdot>p2"
     by (metis assms(1,2) folk_distr2 test_comp_closed_var test_mult_comm_var)
   moreover have "(c\<cdot>d1 + !c\<cdot>d2)\<cdot>(c\<cdot>q1 + !c\<cdot>q2) = c\<cdot>d1\<cdot>c\<cdot>q1 + c\<cdot>d1\<cdot>!c\<cdot>q2 + !c\<cdot>d2\<cdot>c\<cdot>q1 + !c\<cdot>d2\<cdot>!c\<cdot>q2"
-    by (smt add_assoc add_comm mult_distl mult_distr mult_assoc)
+    by (smt add_assoc add_comm distrib_left distrib_right mult_assoc)
   moreover have "... = c\<cdot>d1\<cdot>q1 + !c\<cdot>d2\<cdot>q2"
-    by (metis assms(2-4) kat_double kat_double_zero1 kat_double_zero2 test_comp_closed_var add_zeror)
-  ultimately have one: "(b\<cdot>c + !b\<cdot>!c)\<cdot>(c\<cdot>p1 + !c\<cdot>p2)\<cdot>((c\<cdot>d1 + !c\<cdot>d2)\<cdot>(c\<cdot>q1 + !c\<cdot>q2))\<^sup>*\<cdot>!(c\<cdot>d1 + !c\<cdot>d2)
-                  = (b\<cdot>c\<cdot>p1 + !b\<cdot>!c\<cdot>p2)\<cdot>(c\<cdot>d1\<cdot>q1 + !c\<cdot>d2\<cdot>q2)\<^sup>*\<cdot>(c\<cdot>!d1 + !c\<cdot>!d2)"
-    by (metis assms(2-4) folk_de_morgan2)
-  hence two: "... = (b\<cdot>c\<cdot>p1 + !b\<cdot>!c\<cdot>p2)\<cdot>(c\<cdot>d1\<cdot>q1 + !c\<cdot>d2\<cdot>q2)\<^sup>*\<cdot>c\<cdot>!d1 + (b\<cdot>c\<cdot>p1 + !b\<cdot>!c\<cdot>p2)\<cdot>(c\<cdot>d1\<cdot>q1 + !c\<cdot>d2\<cdot>q2)\<^sup>*\<cdot>!c\<cdot>!d2"
-    by (metis mult_assoc mult_distl)
-  have "(b\<cdot>c\<cdot>p1 + !b\<cdot>!c\<cdot>p2)\<cdot>(c\<cdot>d1\<cdot>q1 + !c\<cdot>d2\<cdot>q2)\<^sup>*\<cdot>c\<cdot>!d1 = b\<cdot>c\<cdot>p1\<cdot>(c\<cdot>d1\<cdot>q1 + !c\<cdot>d2\<cdot>q2)\<^sup>*\<cdot>c\<cdot>!d1 + !b\<cdot>!c\<cdot>p2\<cdot>(c\<cdot>d1\<cdot>q1 + !c\<cdot>d2\<cdot>q2)\<^sup>*\<cdot>c\<cdot>!d1"
-    by (metis mult_distr)
-  moreover have "... = b\<cdot>c\<cdot>p1\<cdot>(d1\<cdot>q1)\<^sup>*\<cdot>!d1 + !b\<cdot>!c\<cdot>p2\<cdot>(c\<cdot>d1\<cdot>q1 + !c\<cdot>d2\<cdot>q2)\<^sup>*\<cdot>c\<cdot>!d1"
+    by (metis assms(2-4) test2 test3 test4 annil test_comp_closed_var add_zeror)
+  ultimately have one: "(b\<cdot>c + !b\<cdot>!c)\<cdot>(c\<cdot>p1 + !c\<cdot>p2)\<cdot>((c\<cdot>d1 + !c\<cdot>d2)\<cdot>(c\<cdot>q1 + !c\<cdot>q2))\<^sup>\<star>\<cdot>!(c\<cdot>d1 + !c\<cdot>d2)
+                  = (b\<cdot>c\<cdot>p1 + !b\<cdot>!c\<cdot>p2)\<cdot>(c\<cdot>d1\<cdot>q1 + !c\<cdot>d2\<cdot>q2)\<^sup>\<star>\<cdot>(c\<cdot>!d1 + !c\<cdot>!d2)"
+    by (metis assms(2-4) de_morgan_var2)
+  hence two: "... = (b\<cdot>c\<cdot>p1 + !b\<cdot>!c\<cdot>p2)\<cdot>(c\<cdot>d1\<cdot>q1 + !c\<cdot>d2\<cdot>q2)\<^sup>\<star>\<cdot>c\<cdot>!d1 + (b\<cdot>c\<cdot>p1 + !b\<cdot>!c\<cdot>p2)\<cdot>(c\<cdot>d1\<cdot>q1 + !c\<cdot>d2\<cdot>q2)\<^sup>\<star>\<cdot>!c\<cdot>!d2"
+    by (metis mult_assoc distrib_left)
+  have "(b\<cdot>c\<cdot>p1 + !b\<cdot>!c\<cdot>p2)\<cdot>(c\<cdot>d1\<cdot>q1 + !c\<cdot>d2\<cdot>q2)\<^sup>\<star>\<cdot>c\<cdot>!d1 = b\<cdot>c\<cdot>p1\<cdot>(c\<cdot>d1\<cdot>q1 + !c\<cdot>d2\<cdot>q2)\<^sup>\<star>\<cdot>c\<cdot>!d1 + !b\<cdot>!c\<cdot>p2\<cdot>(c\<cdot>d1\<cdot>q1 + !c\<cdot>d2\<cdot>q2)\<^sup>\<star>\<cdot>c\<cdot>!d1"
+    by (metis distrib_right)
+  moreover have "... = b\<cdot>c\<cdot>p1\<cdot>(d1\<cdot>q1)\<^sup>\<star>\<cdot>!d1 + !b\<cdot>!c\<cdot>p2\<cdot>(c\<cdot>d1\<cdot>q1 + !c\<cdot>d2\<cdot>q2)\<^sup>\<star>\<cdot>c\<cdot>!d1"
     by (metis assms(1-5,7,8) conditional_helper1 test_comp_closed_var)
-  ultimately have three: "(b\<cdot>c\<cdot>p1 + !b\<cdot>!c\<cdot>p2)\<cdot>(c\<cdot>d1\<cdot>q1 + !c\<cdot>d2\<cdot>q2)\<^sup>*\<cdot>c\<cdot>!d1 = b\<cdot>c\<cdot>p1\<cdot>(d1\<cdot>q1)\<^sup>*\<cdot>!d1"
+  ultimately have three: "(b\<cdot>c\<cdot>p1 + !b\<cdot>!c\<cdot>p2)\<cdot>(c\<cdot>d1\<cdot>q1 + !c\<cdot>d2\<cdot>q2)\<^sup>\<star>\<cdot>c\<cdot>!d1 = b\<cdot>c\<cdot>p1\<cdot>(d1\<cdot>q1)\<^sup>\<star>\<cdot>!d1"
     by (metis assms (1-4,6-8) conditional_helper4 add_zeror)
-  have "(b\<cdot>c\<cdot>p1 + !b\<cdot>!c\<cdot>p2)\<cdot>(c\<cdot>d1\<cdot>q1 + !c\<cdot>d2\<cdot>q2)\<^sup>*\<cdot>!c\<cdot>!d2 = b\<cdot>c\<cdot>p1\<cdot>(c\<cdot>d1\<cdot>q1 + !c\<cdot>d2\<cdot>q2)\<^sup>*\<cdot>!c\<cdot>!d2 + !b\<cdot>!c\<cdot>p2\<cdot>(c\<cdot>d1\<cdot>q1 + !c\<cdot>d2\<cdot>q2)\<^sup>*\<cdot>!c\<cdot>!d2"
-    by (metis mult_distr)
-  moreover have "... = !b\<cdot>!c\<cdot>p2\<cdot>(c\<cdot>d1\<cdot>q1 + !c\<cdot>d2\<cdot>q2)\<^sup>*\<cdot>!c\<cdot>!d2"
+  have "(b\<cdot>c\<cdot>p1 + !b\<cdot>!c\<cdot>p2)\<cdot>(c\<cdot>d1\<cdot>q1 + !c\<cdot>d2\<cdot>q2)\<^sup>\<star>\<cdot>!c\<cdot>!d2 = b\<cdot>c\<cdot>p1\<cdot>(c\<cdot>d1\<cdot>q1 + !c\<cdot>d2\<cdot>q2)\<^sup>\<star>\<cdot>!c\<cdot>!d2 + !b\<cdot>!c\<cdot>p2\<cdot>(c\<cdot>d1\<cdot>q1 + !c\<cdot>d2\<cdot>q2)\<^sup>\<star>\<cdot>!c\<cdot>!d2"
+    by (metis distrib_right)
+  moreover have "... = !b\<cdot>!c\<cdot>p2\<cdot>(c\<cdot>d1\<cdot>q1 + !c\<cdot>d2\<cdot>q2)\<^sup>\<star>\<cdot>!c\<cdot>!d2"
     by (metis assms(1-5,7,8) conditional_helper2 test_comp_closed_var add_zerol)
-  ultimately have four: "(b\<cdot>c\<cdot>p1 + !b\<cdot>!c\<cdot>p2)\<cdot>(c\<cdot>d1\<cdot>q1 + !c\<cdot>d2\<cdot>q2)\<^sup>*\<cdot>!c\<cdot>!d2 = !b\<cdot>!c\<cdot>p2\<cdot>(d2\<cdot>q2)\<^sup>*\<cdot>!d2"
+  ultimately have four: "(b\<cdot>c\<cdot>p1 + !b\<cdot>!c\<cdot>p2)\<cdot>(c\<cdot>d1\<cdot>q1 + !c\<cdot>d2\<cdot>q2)\<^sup>\<star>\<cdot>!c\<cdot>!d2 = !b\<cdot>!c\<cdot>p2\<cdot>(d2\<cdot>q2)\<^sup>\<star>\<cdot>!d2"
     by (metis assms(1-4,6-8) conditional_helper3)
-  have rhs: "(b\<cdot>c + !b\<cdot>!c)\<cdot>(c\<cdot>p1 + !c\<cdot>p2)\<cdot>((c\<cdot>d1 + !c\<cdot>d2)\<cdot>(c\<cdot>q1 + !c\<cdot>q2))\<^sup>*\<cdot>!(c\<cdot>d1 + !c\<cdot>d2) = b\<cdot>c\<cdot>p1\<cdot>(d1\<cdot>q1)\<^sup>*\<cdot>!d1 + !b\<cdot>!c\<cdot>p2\<cdot>(d2\<cdot>q2)\<^sup>*\<cdot>!d2"
+  have rhs: "(b\<cdot>c + !b\<cdot>!c)\<cdot>(c\<cdot>p1 + !c\<cdot>p2)\<cdot>((c\<cdot>d1 + !c\<cdot>d2)\<cdot>(c\<cdot>q1 + !c\<cdot>q2))\<^sup>\<star>\<cdot>!(c\<cdot>d1 + !c\<cdot>d2) = b\<cdot>c\<cdot>p1\<cdot>(d1\<cdot>q1)\<^sup>\<star>\<cdot>!d1 + !b\<cdot>!c\<cdot>p2\<cdot>(d2\<cdot>q2)\<^sup>\<star>\<cdot>!d2"
     by (metis one two three four)
   from lhs and rhs show ?thesis
     by (metis mult_assoc)
@@ -291,32 +159,37 @@ lemma nested_loops_helper: "\<lbrakk>test b; test c\<rbrakk> \<Longrightarrow> (
 proof -
   assume assms: "test b" "test c"
   hence "(b + c)\<cdot>(c\<cdot>q + !c\<cdot>p) = b\<cdot>c\<cdot>q + b\<cdot>!c\<cdot>p + c\<cdot>c\<cdot>q + c\<cdot>!c\<cdot>p"
-    by (metis add_assoc mult_distl mult_distr mult_assoc)
+    by (metis add_assoc distrib_left distrib_right mult_assoc)
   also have "... = b\<cdot>c\<cdot>q + b\<cdot>!c\<cdot>p + c\<cdot>q"
-    by (metis add_comm add_zerol assms(2) mult_annil test_double_comp_var test_mult_comp test_mult_idem_var)
+    by (metis add_0_left add_commute annil assms(2) test_mult_idem_var test_comp_mult)
   also have "... = b\<cdot>c\<cdot>q + c\<cdot>q + !c\<cdot>b\<cdot>p"
     by (metis assms test_comp_closed_var test_mult_comm_var add_assoc add_comm)
   also have "... = (b + 1)\<cdot>c\<cdot>q + !c\<cdot>b\<cdot>p"
-    by (metis mult_distr mult_onel)
+    by (metis distrib_right mult_onel)
   finally show ?thesis
     by (metis add_comm assms(1) mult_onel test_absorb1 test_one_var)
 qed
 
+theorem nested_loops_with_smt: 
+  assumes "test b" "test c"
+  shows "(b\<cdot>p\<cdot>(c\<cdot>q)\<^sup>\<star>\<cdot>!c)\<^sup>\<star>\<cdot>!b = b\<cdot>p\<cdot>((b + c)\<cdot>(c\<cdot>q + !c\<cdot>p))\<^sup>\<star>\<cdot>!(b + c) + !b"
+  by (smt assms nested_loops_helper de_morgan2 mult_assoc star_unfoldl_eq distrib_right mult_onel mult_assoc star_slide star_denest_var assms test_comp_closed_var test_mult_comm_var mult_assoc add_comm )
+
 theorem nested_loops: 
   assumes "test b" "test c"
-  shows "(b\<cdot>p\<cdot>(c\<cdot>q)\<^sup>*\<cdot>!c)\<^sup>*\<cdot>!b = b\<cdot>p\<cdot>((b + c)\<cdot>(c\<cdot>q + !c\<cdot>p))\<^sup>*\<cdot>!(b + c) + !b"
+  shows "(b\<cdot>p\<cdot>(c\<cdot>q)\<^sup>\<star>\<cdot>!c)\<^sup>\<star>\<cdot>!b = b\<cdot>p\<cdot>((b + c)\<cdot>(c\<cdot>q + !c\<cdot>p))\<^sup>\<star>\<cdot>!(b + c) + !b"
 proof -
-  have lhs: "b\<cdot>p\<cdot>((b + c)\<cdot>(c\<cdot>q + !c\<cdot>p))\<^sup>*\<cdot>!(b + c) + !b = b\<cdot>p\<cdot>(c\<cdot>q + !c\<cdot>b\<cdot>p)\<^sup>*\<cdot>!b\<cdot>!c + !b"
+  have lhs: "b\<cdot>p\<cdot>((b + c)\<cdot>(c\<cdot>q + !c\<cdot>p))\<^sup>\<star>\<cdot>!(b + c) + !b = b\<cdot>p\<cdot>(c\<cdot>q + !c\<cdot>b\<cdot>p)\<^sup>\<star>\<cdot>!b\<cdot>!c + !b"
     by (metis assms nested_loops_helper de_morgan2 mult_assoc)
-  have "(b\<cdot>p\<cdot>(c\<cdot>q)\<^sup>*\<cdot>!c)\<^sup>*\<cdot>!b = (1 + b\<cdot>p\<cdot>(c\<cdot>q)\<^sup>*\<cdot>!c\<cdot>(b\<cdot>p\<cdot>(c\<cdot>q)\<^sup>*\<cdot>!c)\<^sup>*)\<cdot>!b"
+  have "(b\<cdot>p\<cdot>(c\<cdot>q)\<^sup>\<star>\<cdot>!c)\<^sup>\<star>\<cdot>!b = (1 + b\<cdot>p\<cdot>(c\<cdot>q)\<^sup>\<star>\<cdot>!c\<cdot>(b\<cdot>p\<cdot>(c\<cdot>q)\<^sup>\<star>\<cdot>!c)\<^sup>\<star>)\<cdot>!b"
     by (metis star_unfoldl_eq)
-  moreover have "... = !b + b\<cdot>p\<cdot>(c\<cdot>q)\<^sup>*\<cdot>!c\<cdot>(b\<cdot>p\<cdot>(c\<cdot>q)\<^sup>*\<cdot>!c)\<^sup>*\<cdot>!b"
-    by (metis mult_distr mult_onel)
-  moreover have "... = !b + b\<cdot>p\<cdot>(c\<cdot>q)\<^sup>*\<cdot>(!c\<cdot>b\<cdot>p\<cdot>(c\<cdot>q)\<^sup>*)\<^sup>*\<cdot>!c\<cdot>!b"
-    by (metis mult_assoc star_sliding)
-  moreover have "(c\<cdot>q + !c\<cdot>b\<cdot>p)\<^sup>* = (c\<cdot>q)\<^sup>*\<cdot>(!c\<cdot>b\<cdot>p\<cdot>(c\<cdot>q)\<^sup>*)\<^sup>*"
-    by (metis star_denesting)
-  ultimately have rhs: "(b\<cdot>p\<cdot>(c\<cdot>q)\<^sup>*\<cdot>!c)\<^sup>*\<cdot>!b = b\<cdot>p\<cdot>(c\<cdot>q + !c\<cdot>b\<cdot>p)\<^sup>*\<cdot>!b\<cdot>!c + !b"
+  moreover have "... = !b + b\<cdot>p\<cdot>(c\<cdot>q)\<^sup>\<star>\<cdot>!c\<cdot>(b\<cdot>p\<cdot>(c\<cdot>q)\<^sup>\<star>\<cdot>!c)\<^sup>\<star>\<cdot>!b"
+    by (metis distrib_right mult_onel)
+  moreover have "... = !b + b\<cdot>p\<cdot>(c\<cdot>q)\<^sup>\<star>\<cdot>(!c\<cdot>b\<cdot>p\<cdot>(c\<cdot>q)\<^sup>\<star>)\<^sup>\<star>\<cdot>!c\<cdot>!b"
+    by (metis mult_assoc star_slide)
+  moreover have "(c\<cdot>q + !c\<cdot>b\<cdot>p)\<^sup>\<star> = (c\<cdot>q)\<^sup>\<star>\<cdot>(!c\<cdot>b\<cdot>p\<cdot>(c\<cdot>q)\<^sup>\<star>)\<^sup>\<star>"
+    by (metis star_denest_var)
+  ultimately have rhs: "(b\<cdot>p\<cdot>(c\<cdot>q)\<^sup>\<star>\<cdot>!c)\<^sup>\<star>\<cdot>!b = b\<cdot>p\<cdot>(c\<cdot>q + !c\<cdot>b\<cdot>p)\<^sup>\<star>\<cdot>!b\<cdot>!c + !b"
     by (metis assms test_comp_closed_var test_mult_comm_var mult_assoc add_comm)
   from lhs and rhs show ?thesis
     by metis
@@ -330,24 +203,24 @@ text {*
 *}
 theorem postcomputation: 
   assumes "test b" "p\<cdot>b = b\<cdot>p" "q\<cdot>b = b\<cdot>q" 
-  shows "(b\<cdot>p)\<^sup>*\<cdot>!b\<cdot>q = !b\<cdot>q + b\<cdot>(b\<cdot>p\<cdot>(!b\<cdot>q + b))\<^sup>*\<cdot>!b"
+  shows "(b\<cdot>p)\<^sup>\<star>\<cdot>!b\<cdot>q = !b\<cdot>q + b\<cdot>(b\<cdot>p\<cdot>(!b\<cdot>q + b))\<^sup>\<star>\<cdot>!b"
 proof -
-  have lhs: "(b\<cdot>p)\<^sup>*\<cdot>!b\<cdot>q = !b\<cdot>q + b\<cdot>p\<cdot>(b\<cdot>p)\<^sup>*\<cdot>!b\<cdot>q"
-    by (metis mult_distr mult_onel star_def star_transl)
-  have "b\<cdot>(b\<cdot>p\<cdot>(!b\<cdot>q + b))\<^sup>*\<cdot>!b = b\<cdot>!b + b\<cdot>b\<cdot>p\<cdot>(!b\<cdot>q + b)\<cdot>(b\<cdot>p\<cdot>(!b\<cdot>q + b))\<^sup>*\<cdot>!b"
-    by (metis mult_distl mult_distr mult_oner mult_assoc star_unfoldl_eq)
-  also have "... = b\<cdot>p\<cdot>(!b\<cdot>q + b)\<cdot>(b\<cdot>p\<cdot>(!b\<cdot>q + b))\<^sup>*\<cdot>!b" 
-    by (metis assms(1) ba6 comm_eq3 add_zerol test_mult_idem_var)
-  also have "... = b\<cdot>p\<cdot>((!b\<cdot>q + b)\<cdot>b\<cdot>p)\<^sup>*\<cdot>(!b\<cdot>q + b)\<cdot>!b" 
+  have lhs: "(b\<cdot>p)\<^sup>\<star>\<cdot>!b\<cdot>q = !b\<cdot>q + b\<cdot>p\<cdot>(b\<cdot>p)\<^sup>\<star>\<cdot>!b\<cdot>q"
+    by (metis add_commute mult_1_left mult_assoc star_invol star_one star_prod_unfold star_slide star_trans_eq troeger)
+  have "b\<cdot>(b\<cdot>p\<cdot>(!b\<cdot>q + b))\<^sup>\<star>\<cdot>!b = b\<cdot>!b + b\<cdot>b\<cdot>p\<cdot>(!b\<cdot>q + b)\<cdot>(b\<cdot>p\<cdot>(!b\<cdot>q + b))\<^sup>\<star>\<cdot>!b"
+    by (metis distrib_left distrib_right mult_oner mult_assoc star_unfoldl_eq)
+  also have "... = b\<cdot>p\<cdot>(!b\<cdot>q + b)\<cdot>(b\<cdot>p\<cdot>(!b\<cdot>q + b))\<^sup>\<star>\<cdot>!b" 
+    by (metis add_zerol assms(1) test_comp_mult test_mult_idem_var)
+  also have "... = b\<cdot>p\<cdot>((!b\<cdot>q + b)\<cdot>b\<cdot>p)\<^sup>\<star>\<cdot>(!b\<cdot>q + b)\<cdot>!b" 
     by (metis mult_assoc star_slide)
-  also have "... = b\<cdot>p\<cdot>((!b\<cdot>q\<cdot>b + b\<cdot>b)\<cdot>p)\<^sup>*\<cdot>(!b\<cdot>q\<cdot>!b + b\<cdot>!b)"
-    by (metis mult_distr mult_assoc)
-  also have "... = b\<cdot>p\<cdot>((!b\<cdot>q\<cdot>b + b)\<cdot>p)\<^sup>*\<cdot>(!b\<cdot>q\<cdot>!b)"
-    by (metis assms(1) ba6 comm_eq3 add_zeror test_mult_idem_var)
-  also have "... = b\<cdot>p\<cdot>((!b\<cdot>b\<cdot>q + b)\<cdot>p)\<^sup>*\<cdot>(!b\<cdot>!b\<cdot>q)"
+  also have "... = b\<cdot>p\<cdot>((!b\<cdot>q\<cdot>b + b\<cdot>b)\<cdot>p)\<^sup>\<star>\<cdot>(!b\<cdot>q\<cdot>!b + b\<cdot>!b)"
+    by (metis distrib_right mult_assoc)
+  also have "... = b\<cdot>p\<cdot>((!b\<cdot>q\<cdot>b + b)\<cdot>p)\<^sup>\<star>\<cdot>(!b\<cdot>q\<cdot>!b)"
+    by (smt add_0_left add_commute assms(1) test_mult_idem_var test_comp_mult)
+  also have "... = b\<cdot>p\<cdot>((!b\<cdot>b\<cdot>q + b)\<cdot>p)\<^sup>\<star>\<cdot>(!b\<cdot>!b\<cdot>q)"
     by (metis assms(1,3) comm_eq3 mult_assoc)
-  finally have rhs: "b\<cdot>(b\<cdot>p\<cdot>(!b\<cdot>q + b))\<^sup>*\<cdot>!b = b\<cdot>p\<cdot>(b\<cdot>p)\<^sup>*\<cdot>(!b\<cdot>q)"
-    by (metis assms(1) ba6 mult_assoc mult_annil add_zerol test_comp_closed_var test_mult_idem_var)
+  finally have rhs: "b\<cdot>(b\<cdot>p\<cdot>(!b\<cdot>q + b))\<^sup>\<star>\<cdot>!b = b\<cdot>p\<cdot>(b\<cdot>p)\<^sup>\<star>\<cdot>(!b\<cdot>q)"
+    by (metis add_0_right add_commute annil assms(1) ba6 assms(1) test_mult_idem test_def)
   from lhs and rhs show ?thesis
     by (metis mult_assoc)
 qed
@@ -360,11 +233,11 @@ text {*
 *}
 theorem composition:
   assumes "test b" "test c" "p\<cdot>b = b\<cdot>p" "q\<cdot>b = b\<cdot>q" 
-  shows "(b\<cdot>p)\<^sup>*\<cdot>!b\<cdot>(c\<cdot>q)\<^sup>*\<cdot>!c = !b\<cdot>(c\<cdot>q)\<^sup>*\<cdot>!c + b\<cdot>(b\<cdot>p\<cdot>(!b\<cdot>(c\<cdot>q)\<^sup>*\<cdot>!c + b))\<^sup>*\<cdot>!b"
+  shows "(b\<cdot>p)\<^sup>\<star>\<cdot>!b\<cdot>(c\<cdot>q)\<^sup>\<star>\<cdot>!c = !b\<cdot>(c\<cdot>q)\<^sup>\<star>\<cdot>!c + b\<cdot>(b\<cdot>p\<cdot>(!b\<cdot>(c\<cdot>q)\<^sup>\<star>\<cdot>!c + b))\<^sup>\<star>\<cdot>!b"
 proof -
-  let ?x = "(c\<cdot>q)\<^sup>*\<cdot>!c"
+  let ?x = "(c\<cdot>q)\<^sup>\<star>\<cdot>!c"
   have "b\<cdot>?x = ?x\<cdot>b"
-    by (metis assms(1,2,4) comm_eq5 comm_mult mult_assoc test_comp_closed_var test_mult_comm_var)
+    by (metis assms(1,2,4) star_sim3 comm_mult mult_assoc test_comp_closed_var test_mult_comm_var)
   thus ?thesis
     by (metis assms(1,3) mult_assoc postcomputation)
 qed
